AsyncDisk and DiskSSM

concurrency/framework/AsyncDisk.s.dfy
@@ -5,46 +5,31 @@ module DiskIfc refines Ifc {
   import opened NativeTypes
   import opened RequestIds
 
-  datatype ReqRead = ReqRead(addr: uint64, len: uint64)
-  datatype ReqWrite = ReqWrite(addr: uint64, bytes: seq<byte>)
-  datatype RespRead = RespRead(addr: uint64, bytes: seq<byte>)
-  datatype RespWrite = RespWrite(addr: uint64, len: uint64)
+  datatype ReqRead = ReqRead(addr: int, len: int)
+  datatype ReqWrite = ReqWrite(addr: int, bytes: seq<byte>)
+  datatype RespRead = RespRead(addr: int, bytes: seq<byte>)
+  datatype RespWrite = RespWrite(addr: int, len: int)
 
   datatype DiskOp =
     | ReqReadOp(id: RequestId, reqRead: ReqRead)
     | ReqWriteOp(id: RequestId, reqWrite: ReqWrite)
     | RespReadOp(id: RequestId, respRead: RespRead)
     | RespWriteOp(id: RequestId, respWrite: RespWrite)
-    | NoDiskOp
 
   type Op = DiskOp
 }
 
 module AsyncDisk refines StateMachine(DiskIfc) {
   import opened NativeTypes
-
   import opened DiskIfc
-
-  type ReqId = uint64
-
-  datatype ReqRead = ReqRead(addr: uint64, len: uint64)
-  datatype ReqWrite = ReqWrite(addr: uint64, bytes: seq<byte>)
-  datatype RespRead = RespRead(addr: uint64, bytes: seq<byte>)
-  datatype RespWrite = RespWrite(addr: uint64, len: uint64)
-
-  datatype DiskOp =
-    | ReqReadOp(id: ReqId, reqRead: ReqRead)
-    | ReqWriteOp(id: ReqId, reqWrite: ReqWrite)
-    | RespReadOp(id: ReqId, respRead: RespRead)
-    | RespWriteOp(id: ReqId, respWrite: RespWrite)
-    | NoDiskOp
+  import opened RequestIds
 
   datatype Variables = Variables(
     // Queue of requests and responses:
-    reqReads: map<ReqId, ReqRead>,
-    reqWrites: map<ReqId, ReqWrite>,
-    respReads: map<ReqId, RespRead>,
-    respWrites: map<ReqId, RespWrite>,
+    reqReads: map<RequestId, ReqRead>,
+    reqWrites: map<RequestId, ReqWrite>,
+    respReads: map<RequestId, RespRead>,
+    respWrites: map<RequestId, RespWrite>,
 
     // The disk:
     contents: seq<byte>
@@ -63,7 +48,6 @@ module AsyncDisk refines StateMachine(DiskIfc) {
     | RecvWriteStep
     | AckReadStep
     | AckWriteStep
-    | StutterStep
 
   predicate RecvRead(s: Variables, s': Variables, dop: DiskOp)
   {
@@ -97,19 +81,12 @@ module AsyncDisk refines StateMachine(DiskIfc) {
     && s' == s.(respWrites := s.respWrites - {dop.id})
   }
 
-  predicate Stutter(s: Variables, s': Variables, dop: DiskOp)
-  {
-    && dop.NoDiskOp?
-    && s' == s
-  }
-
   predicate NextStep(s: Variables, s': Variables, dop: DiskOp, step: Step) {
     match step {
       case RecvReadStep => RecvRead(s, s', dop)
       case RecvWriteStep => RecvWrite(s, s', dop)
       case AckReadStep => AckRead(s, s', dop)
       case AckWriteStep => AckWrite(s, s', dop)
-      case StutterStep => Stutter(s, s', dop)
     }
   }
 
@@ -118,17 +95,17 @@ module AsyncDisk refines StateMachine(DiskIfc) {
   }
 
   datatype InternalStep =
-    | ProcessReadStep(id: ReqId)
-    | ProcessWriteStep(id: ReqId)
-    | HavocConflictingWritesStep(id: ReqId, id': ReqId)
-    | HavocConflictingWriteReadStep(id: ReqId, id': ReqId)
+    | ProcessReadStep(id: RequestId)
+    | ProcessWriteStep(id: RequestId)
+    | HavocConflictingWritesStep(id: RequestId, id': RequestId)
+    | HavocConflictingWriteReadStep(id: RequestId, id': RequestId)
 
-  predicate ProcessRead(s: Variables, s': Variables, id: ReqId)
+  predicate ProcessRead(s: Variables, s': Variables, id: RequestId)
   {
     && id in s.reqReads
     && var req := s.reqReads[id];
     && 0 <= req.addr as int <= req.addr as int + req.len as int <= |s.contents|
-    && s' == s.(reqReads := MapRemove1(s.reqReads, id))
+    && s' == s.(reqReads := s.reqReads - {id})
               .(respReads := s.respReads[id := RespRead(req.addr, s.contents[req.addr .. req.addr as int + req.len as int])])
   }
 
@@ -139,15 +116,15 @@ module AsyncDisk refines StateMachine(DiskIfc) {
     bytes[.. start] + ins + bytes[start + |ins| ..]
   }
 
-  predicate ProcessWrite(s: Variables, s': Variables, id: ReqId)
+  predicate ProcessWrite(s: Variables, s': Variables, id: RequestId)
   {
     && id in s.reqWrites
     && var req := s.reqWrites[id];
     && 0 <= req.addr
     && |req.bytes| < 0x1_0000_0000_0000_0000
     && req.addr as int + |req.bytes| <= |s.contents|
-    && s' == s.(reqWrites := MapRemove1(s.reqWrites, id))
-              .(respWrites := s.respWrites[id := RespWrite(req.addr, |req.bytes| as uint64)])
+    && s' == s.(reqWrites := s.reqWrites - {id})
+              .(respWrites := s.respWrites[id := RespWrite(req.addr, |req.bytes| as int)])
               .(contents := splice(s.contents, req.addr as int, req.bytes))
   }
 
@@ -160,7 +137,7 @@ module AsyncDisk refines StateMachine(DiskIfc) {
     && start' + len' > start
   }
 
-  predicate HavocConflictingWrites(s: Variables, s': Variables, id: ReqId, id': ReqId)
+  predicate HavocConflictingWrites(s: Variables, s': Variables, id: RequestId, id': RequestId)
   {
     && id != id'
     && id in s.reqWrites
@@ -170,7 +147,7 @@ module AsyncDisk refines StateMachine(DiskIfc) {
         s.reqWrites[id'].addr as int, |s.reqWrites[id'].bytes|)
   }
 
-  predicate HavocConflictingWriteRead(s: Variables, s': Variables, id: ReqId, id': ReqId)
+  predicate HavocConflictingWriteRead(s: Variables, s': Variables, id: RequestId, id': RequestId)
   {
     && id in s.reqWrites
     && id' in s.reqReads
@@ -182,8 +159,7 @@ module AsyncDisk refines StateMachine(DiskIfc) {
   predicate NextInternalStep(s: Variables, s': Variables, step: InternalStep)
   {
     match step {
-      //case ProcessReadStep(id) => ProcessRead(s, s', id)
-      case ProcessReadFailureStep(id, fakeContents) => ProcessReadFailure(s, s', id, fakeContents)
+      case ProcessReadStep(id) => ProcessRead(s, s', id)
       case ProcessWriteStep(id) => ProcessWrite(s, s', id)
       case HavocConflictingWritesStep(id, id') => HavocConflictingWrites(s, s', id, id')
       case HavocConflictingWriteReadStep(id, id') => HavocConflictingWriteRead(s, s', id, id')
