concurrency/framework/DiskSSM.s.dfy
@@ -1,5 +1,6 @@
 include "PCM.s.dfy"
 include "StateMachines.s.dfy"
+include "AsyncDisk.s.dfy"
 include "../../lib/Lang/NativeTypes.s.dfy"
 
 abstract module DiskSSM(IOIfc: InputOutputIfc) {
@@ -20,9 +21,9 @@ abstract module DiskSSM(IOIfc: InputOutputIfc) {
   function request_ids_in_use(m: M) : set<RequestId>
 
   function DiskWriteReq(disk_addr: int, data: seq<byte>) : M
-  function DiskWriteResp(disk_addr: int) : M
+  function DiskWriteResp(disk_addr: int, len: int) : M
 
-  function DiskReadReq(disk_addr: int) : M
+  function DiskReadReq(disk_addr: int, len: int) : M
   function DiskReadResp(disk_addr: int, data: seq<byte>) : M
 
   predicate Init(s: M)
@@ -59,12 +60,12 @@ abstract module DiskSSM(IOIfc: InputOutputIfc) {
   ensures Inv(whole')
 
   lemma ProcessReadPreservesInv(disk_addr: int, data: seq<byte>, rest: M)
-  requires Inv(dot(DiskReadReq(disk_addr), rest))
+  requires Inv(dot(DiskReadReq(disk_addr, |data|), rest))
   ensures Inv(dot(DiskReadResp(disk_addr, data), rest))
 
   lemma ProcessWritePreservesInv(disk_addr: int, data: seq<byte>, rest: M)
   requires Inv(dot(DiskWriteReq(disk_addr, data), rest))
-  ensures Inv(dot(DiskWriteResp(disk_addr), rest))
+  ensures Inv(dot(DiskWriteResp(disk_addr, |data|), rest))
 
   lemma dot_unit(x: M)
   ensures dot(x, unit()) == x
@@ -80,31 +81,117 @@ abstract module DiskSSM(IOIfc: InputOutputIfc) {
   ensures Inv(s)
 }
 
-module TicketStubStateMachine(IOIfc: InputOutputIfc, ssm: TicketStubSSM(IOIfc))
-    refines StateMachine(AsyncIfc(IOIfc))
+module CrashAsyncIfc(ifc: InputOutputIfc) refines Ifc {
+  import opened RequestIds
+
+  datatype Op =
+    | Start(rid: RequestId, input: ifc.Input)
+    | End(rid: RequestId, output: ifc.Output)
+    | InternalOp
+    | CrashOp
+}
+
+module AsyncDiskSystemStateMachine(IOIfc: InputOutputIfc, ssm: DiskSSM(IOIfc))
+    refines StateMachine(CrashAsyncIfc(IOIfc))
 {
   import AsyncIfc = AsyncIfc(IOIfc)
+  import Disk = AsyncDisk
+  import opened DiskIfc
+  import opened RequestIds
 
-  type Variables = ssm.M
+  datatype Variables = Variables(
+      disk: Disk.Variables,
+      machine: ssm.M)
 
   predicate Init(s: Variables) {
-    ssm.Init(s)
+    && Disk.Init(s.disk)
+    && ssm.Init(s.machine)
   }
 
-  predicate InternalNext(s: Variables, s': Variables,
+  /*predicate InternalNext(s: Variables, s': Variables,
       shard: Variables, shard': Variables, rest: Variables)
   {
     && s == ssm.dot(shard, rest)
     && s' == ssm.dot(shard', rest)
     && ssm.Internal(shard, shard')
+  }*/
+
+  predicate Crash(s: Variables, s': Variables)
+  {
+    && Disk.Crash(s.disk, s'.disk)
+    && ssm.Init(s'.machine)
+  }
+
+  datatype Step =
+    | MachineStep(shard: ssm.M, shard': ssm.M, rest: ssm.M)
+    | InteractionStep(dop: DiskOp)
+    | DiskInternalStep
+
+  predicate Machine(s: Variables, s': Variables, shard: ssm.M, shard': ssm.M, rest: ssm.M) {
+    && ssm.Internal(shard, shard')
+    && s.machine == ssm.dot(shard, rest)
+    && s'.machine == ssm.dot(shard', rest)
+    && s'.disk == s.disk
+  }
+
+  predicate DiskInternal(s: Variables, s': Variables) {
+    && s.machine == s'.machine
+    && Disk.NextInternal(s.disk, s'.disk)
+  }
+
+  predicate MachineInteraction(s: ssm.M, s': ssm.M, dop: DiskOp) {
+    match dop {
+      case ReqReadOp(id, reqRead) =>
+        s == ssm.dot(s', ssm.DiskReadReq(reqRead.addr, reqRead.len))
+
+      case ReqWriteOp(id, reqWrite) =>
+        s == ssm.dot(s', ssm.DiskWriteReq(reqWrite.addr, reqWrite.bytes))
+
+      case RespReadOp(id, respRead) =>
+        s' == ssm.dot(s, ssm.DiskReadResp(respRead.addr, respRead.bytes))
+
+      case RespWriteOp(id, respWrite) =>
+        s' == ssm.dot(s, ssm.DiskWriteResp(respWrite.addr, respWrite.len))
+    }
+  }
+
+  predicate Interaction(s: Variables, s': Variables, dop: DiskOp) {
+    && Disk.Next(s.disk, s'.disk, dop)
+    && MachineInteraction(s.machine, s'.machine, dop)
+  }
+
+  predicate InternalStep(s: Variables, s': Variables, step: Step)
+  {
+    match step {
+      case MachineStep(shard, shard', rest) => Machine(s, s', shard, shard', rest)
+      case InteractionStep(dop) => Interaction(s, s', dop)
+      case DiskInternalStep => DiskInternal(s, s')
+    }
+  }
+
+  predicate Internal(s: Variables, s': Variables)
+  {
+    exists step :: InternalStep(s, s', step)
+  }
+
+  predicate NewTicket(s: Variables, s': Variables, rid: RequestId, input: IOIfc.Input)
+  {
+    && ssm.NewTicket(s.machine, s'.machine, rid, input)
+    && s.disk == s'.disk
+  }
+
+  predicate ConsumeStub(s: Variables, s': Variables, rid: RequestId, output: IOIfc.Output)
+  {
+    && ssm.ConsumeStub(s.machine, s'.machine, rid, output)
+    && s.disk == s'.disk
   }
 
   predicate Next(s: Variables, s': Variables, op: ifc.Op) {
     match op {
-      case Start(rid, input) => ssm.NewTicket(s, s', rid, input)
-      case End(rid, output) => ssm.ConsumeStub(s, s', rid, output)
-      case InternalOp =>
-        exists shard, shard', rest :: InternalNext(s, s', shard, shard', rest)
+      case Start(rid, input) => NewTicket(s, s', rid, input)
+      case End(rid, output) => ConsumeStub(s, s', rid, output)
+      case CrashOp => Crash(s, s')
+      case InternalOp => Internal(s, s')
     }
   }
 }
